\documentclass[12pt]{article}
\usepackage[utf8x]{inputenc}
\usepackage[english]{babel}
\usepackage[T1]{fontenc}
\usepackage{wrapfig}
\usepackage{amsmath}
\usepackage{amssymb}
\usepackage[font=small,format=plain,labelfont=bf,up,textfont=it,up]{caption}
\usepackage{calc}
\usepackage{ifthen}
\usepackage{relsize}
\usepackage{bbold}
\usepackage{mathtext}
\usepackage{pdfpages}
\usepackage{geometry}
 \geometry{
 a4paper,
 total={170mm,257mm},
 left=35mm,
 top=25mm,
 bottom=25mm,
 right=20mm,
 }

\begin{document}
\noindent Suppose we have two unpaired electrons. The two-particle Hilbert space spanned by

\begin{equation}
|s_{1}m_{1}\rangle \otimes | s_{2}m_{2} \rangle = | s_{1}m_{1}, s_{2}m_{2} \rangle,
\end{equation}

\noindent the RHS is just a short hand of writing one of the vectors formed from the product $\otimes$. From now on this will be referred to as the \emph{product basis} . \\

\noindent The particles have spin operators denoted $\hat{S}_{1}$ and $\hat{S}_{2}$. The product
states satisfy

\noindent As $m_{1}  \text{and} m_{2} = \pm \frac{1}{2} $, we shall use the further shorthand, e.g.,
the product state for $s_{1,2} = \frac{1}{2}$, $m_{1} = +\frac{1}{2}$ and $m_{2} = -\frac{1}{2} $ 
will be written
\begin{equation}
|+-\rangle = | \frac{1}{2}\frac{1}{2},\frac{1}{2}\frac{-1}{2} \rangle
\end{equation}
\begin{equation}
S^{2}_{i}|s_{1}m_{1}, s_{2}m_{2} \rangle = \hbar^{2}s_{i}(s+1)|s_{1}m_{1}, s_{2}m_{2} \rangle
\end{equation}
\noindent The total angular momentum operator, $\mathbf{S}$, is defined 
\begin{equation}
\mathbf{S} = \mathbf{S}_{1}+\mathbf{S}_{2}
\end{equation}
We want to find the eigenvalues of $S_{z}$ and $S^{2}$ in this basis. First, look at
$S_{z}$.
\begin{equation}
S_{z}|++\rangle =
(S_{1z}+S_{2z})|++ = (\frac{\hbar}{2} + \frac{\hbar}{2}) | ++ rangle = |++\rangle
\end{equation}
\begin{equation}
S_{z}|++\rangle =
(S_{1z}+S_{2z})|++ = (\frac{-\hbar}{2} + \frac{\hbar}{2}) | -+ rangle = 0
\end{equation}
\begin{equation}
S_{z}|++\rangle =
(S_{1z}+S_{2z})|++ = (\frac{\hbar}{2} + \frac{-\hbar}{2}) | +- rangle = 0
\end{equation}
\begin{equation}
S_{z}|++\rangle = 
(S_{1z}+S_{2z})|++ = (\frac{-\hbar}{2} + \frac{-\hbar}{2}) | -- \rangle = | -- \rangle
\end{equation}
So the representation of $\mathbf{S}_{z}$ in the product basis is
\begin{equation}
[S_{z}]_{\{|1,2\rangle\}} = 
\begin{bmatrix}
1                  & 0 & 0 & 0 \\
0                  & 0 & 0 & 0 \\
0                  & 0 & 0 & 0 \\
0                  & 0 & 0 & -1 
\end{bmatrix}
\end{equation}
where the $\hbar$ has been omitted for convenience.\\

\noindent Now consider the $S^{2}$ operator. 
\begin{equation}
S^{2} = (\mathbf{S}_{1}+\mathbf{S}_{2})\cdot (\mathbf{S}_{1}+\mathbf{S}_{2})= 
S^{2}_{1}+S^{2}_{2} + 2\mathbf{S}_{1}\cdot \mathbf{S}_{2}
\end{equation}
\noindent Unfortunately, the product states are not eigenfunctions of $S^{2}$. This
leads us to construct the following basis:
\begin{equation*}
\frac{|+-\rangle - | -+ \rangle}{\sqrt{2}}
\end{equation*}
\\
\begin{equation*}
|++\rangle
\end{equation*}
\begin{equation*}
\frac{|+-\rangle - | -+ \rangle}{\sqrt{2}}
\end{equation*}
\begin{equation*}
|--\rangle
\end{equation*}
\noindent I'll refer to this as the "ST basis". The question is now which of these two bases should we use. If 
we are interested in and operator, $\hat{V}^{(+)}$ of the form,
\begin{equation}
\hat{V}^{(+)} = -(v^{(+)}_{1}\mathbf{S}_{1} + v^{(+)}_{2}\mathbf{S}_{2}) \cdot \mathbf{B}
\end{equation}
this indicates non-interacting spins, hence it makes sense to use the product basis.
However, if we have and operator $\hat{V}^{\times}$, corresponding to 
interacting spins
\begin{equation}
\hat{V}^{\times} = v^{\times}\mathbf{S}_{1}\cdot\mathbf{S}_{2}
\end{equation}
then it makes send to use the ST basis.\\

\noindent Soncini provides a basis of matrices which may be used to represent 
the representation of an operator in the above bases. To understand how
this basis is constructed, it is useful to recap the addition of angular momentum,
and how bases such as those above can be transformed into one another. 

\section{Addition of classical angular momentum}
Consider adding two angular momenta, and the associated product states. As
with spin we have
\begin{equation}
J_{z}|j_{1}m_{1} \rangle = (m_{1}+m_{2})|j_{1}m_{1}, j_{2}m_{2} \rangle
\end{equation}
Note that his is going to be degenrate, as multiple combinations of $m_{1}$ and $m_{2}$
can result in the same eigenvalue. Within each of these degenerate eigenspaces 
(which can be thought of corresponding to spin multiplets) we want to chose a 
basis which consists solely of eigenvectors of $J^{2}$.\\

\noindent If $j_{1}\geq j_{2}$, then the value of the total angular momentum $j$ can
take on values 
\begin{equation}
(j_{1}+j_{2}-1), (j_{1}+j_{2}-2), ... , (j_{1}-j_{2})
\end{equation}
\noindent So the total number of states in this basis is $(2j_{1}+1)(2j_{2}+1)$.
In fact we can state that the tensor product space $j_{1}\otimes j_{2}$ can
be represented as a sum of spaces, each of which is associated with one the 
eigenvalues stated above, i.e.,
\begin{equation}
j_{1}\otimes j_{2} =
(j_{1}+j_{2})\oplus
(j_{1}+j_{2}-1)\oplus
...
(j_{1}-j_{2})
\end{equation}
The states within each one of these degenerate subspaces are
\begin{equation}
|JM, j_{1}j_{2} \rangle 
\text{ \ \ where \ \ } (j_{1}+j_{2}) \geq j \geq (j_{1}-j_{2})
\text{ \ \ and \ \  } j\geq m \geq -j
\end{equation}
Now we can consider which states exist in each one of these degenerate subspaces
\begin{table}[]
\begin{tabular}{@{}llllll@{}}
\hline
\multicolumn{1}{l||}{}     & \multicolumn{1}{l|}{$J=j_{1}+j_{2}$} & \multicolumn{1}{l|}{$J=j_{1}+j_{2}-1$}      & \multicolumn{1}{l|}{$J=j_{1}+j_{2}-2$} & \multicolumn{1}{l}{$J=j_{1}+j_{2}-3$} \\
\hline\hline
\multicolumn{1}{l||}{m=3}  & \multicolumn{1}{l|}{$|3,3\rangle$}  &  \multicolumn{1}{l|}{} & \multicolumn{1}{l|}{} & \multicolumn{1}{l}{}               & \multicolumn{1}{l}{}              \\
\multicolumn{1}{l||}{m=2}  & \multicolumn{1}{l|}{$|3,2\rangle $} &  \multicolumn{1}{l|}{$|2,2\rangle$ }           & \multicolumn{1}{l|}{}               & \multicolumn{1}{l}{}              \\
\multicolumn{1}{l||}{m=1}  & \multicolumn{1}{l|}{$|3,1\rangle $} &  \multicolumn{1}{l|}{$|2,1\rangle$ }           & \multicolumn{1}{l|}{$|1,1\rangle $} & \multicolumn{1}{l}{}              \\
\multicolumn{1}{l||}{m=0}  & \multicolumn{1}{l|}{$|3,0\rangle $} &  \multicolumn{1}{l|}{$|2,0\rangle$ }           & \multicolumn{1}{l|}{$|1,0\rangle $} & \multicolumn{1}{l}{$|0,0\rangle $}  \\
\multicolumn{1}{l||}{M=-1} & \multicolumn{1}{l|}{$|3,-1\rangle$} & \multicolumn{1}{l|} {$|2,-1\rangle$ }          & \multicolumn{1}{l|}{$|1,-1\rangle$} & \multicolumn{1}{l}{}              \\
\multicolumn{1}{l||}{M=-2} & \multicolumn{1}{l|}{$|3,-2\rangle$} & \multicolumn{1}{l|} {$|2,-2\rangle$ }          & \multicolumn{1}{l|}{}               & \multicolumn{1}{l}{}              \\
\multicolumn{1}{l||}{M=-3} & \multicolumn{1}{l|}{$|3,-3\rangle$} & \multicolumn{1}{l|}{} & \multicolumn{1}{l|}{}  & \multicolumn{1}{l}{}               & \multicolumn{1}{l}{} 
\end{tabular}
\end{table}
Or, when applied to the $j_{1} = j_{2} = \frac{1}{2}$ case we have
\begin{table}[]
\begin{tabular}{@{}llllll@{}}
\hline
\multicolumn{1}{l||}{}     &   \multicolumn{1}{l|}{$J= 1 $} & \multicolumn{1}{l}{$J=0$} \\
\hline\hline
\multicolumn{1}{l||}{m=1}  &    \multicolumn{1}{l|}{$|1,1\rangle $} & \multicolumn{1}{l}{}              \\
\multicolumn{1}{l||}{m=0}  &    \multicolumn{1}{l|}{$|1,0\rangle $} & \multicolumn{1}{l}{$|0,0\rangle $}  \\
\multicolumn{1}{l||}{M=-1} &     \multicolumn{1}{l|}{$|1,-1\rangle$} & \multicolumn{1}{l}{}              \\
\end{tabular}
\end{table}
It must be possible to obtain these states (which have a good value of $J^{2}$)
via some transformation of the states in the product basis. We can see that for
the $|S=1,M=1\rangle$ state in the product basis is the same as the state in
the ST basis. We can now generate the other states via use of the ladder
operators on this high spin state, i.e.,
\begin{equation*}
\hat{S}_{-} | 1,1\rangle = \frac{1}{\sqrt{2}}|1,0\rangle 
\end{equation*}
\begin{equation*}
= (\hat{s}_{1-}+\hat{s}_{2-}) | 1,1\rangle = \frac{1}{\sqrt{2}}(|+-\rangle + |-+\rangle)
\end{equation*}
acting again with the ladder operator yields
\begin{equation}
S_{-1}|S=1,M=0\rangle  = |--\rangle
\end{equation}
Whilst this proeedure is done for the simple case of two similar spins of $\frac{1}{2}$, is it can
be applied generally to any angualr momenta, and hence may be applied recursively to build up
systems of more than two couple momenta. For example, the appropriate basis for three coupled spins can be 
obtained by first constructing the ST basis for two coupled spins, and then coupling a further third
spin to the states in this ST basis.\\

\noindent A side note is that the choice of phase for these spins can alter the sign resulting 
from application of the ladder operators. It is important to bear this in mind, but generally, the
phase is chose so that the signs yielded are those shown above.\\

\noindent We now need to consider $|S=0, M=0\rangle$. This can be obtained by noting 
it must be orthogonal to the above defined states. By convention, it is also chosen such that it
has real coefficients (I don't know if this convention has any significant ramifications, or requires justificaiton).
We also require it to be normalized to 1. Orthogonality to $|++\rangle$ and $|--\rangle$ means
the state must be written as some combination
\begin{equation}
|0,0\rangle = \alpha | +-\rangle +\beta| -+\rangle
 \text{\ \ \ where \ \ } \alpha+\beta =0
 \text{ \ \ \ and \ \ \ } \alpha^{2}+\beta^{2} = 1
\end{equation}
Solving for $\alpha$ and $\beta$ yields
\begin{equation}
|0,0\rangle = \frac{1}{\sqrt{2}} (|+-\rangle - | -+\rangle )
\end{equation}
the standard covention is that the coefficient corresponding to the state with
$m_{1} = j_{1}$ positive for the $|J=0, M=0\rangle$ state. Again this doesn't 
truly matter, but is important if we want our coefficients to match up 
with everyone elses.\\

\noindent We can now think about extending this to the general problem, i.e., the case
where $j_{1}$ and $j_{2}$ take any value (where we chose the indexes so $j_{1} \geq j_{2}$). 
As before, the state with the highest angular momenta ($J=j_{1}+j_{2}$) is the same as
can be built out of a single product ket 
\begin{equation}
|J= (j_{1}+j_{2}), M=(j_{1}+j_{2})\rangle = | j_{1} =j_{1}, m_{1}=j_{1}; j_{2}=j_{2},m_{2}=j_{2} \rangle 
\end{equation}
\noindent  As before we can use the ladder operators to decrease the value of $M$ one step
\begin{equation}
|J= (j_{1}+j_{2}), M=(j_{1}+j_{2})\rangle =
\frac{1}{\hbar}J_{-}|J= (j_{1}+j_{2}), M=(j_{1}+j_{2})\rangle 
\end{equation}
\noindent hence
\begin{equation*}
| j_{1}+j_{2}, j_{1}+j_{2}-1\rangle
=\sqrt{\frac{1}{2(j_{1}+j_{2})}}(J_{1-}+J_{2-})|J,M\rangle
\end{equation*}
%\begin{equation*}
%=\sqrt{\frac{1}{2(j_{1}+j_{2})}}(J_{1-}+J_{2-}) (|j_{1}= j_{1},j_{2}=(j_{2}-1)\rangle + |j_{1}=(j_{1}-1),j_{2}=j_{2}\rangle)
%\end{equation*}
\begin{equation*}
J=| j_{1}+j_{2},M= j_{1}+j_{2}-1\rangle
=\sqrt{\frac{j_{1}}{j_{1}+j_{2}}}  \Bigg|j_{1}= (j_{1}-1) ,j_{2}=j_{2}\Bigg\rangle+
 \sqrt{\frac{j_{2}}{j_{1}+j_{2}}}  \Bigg|j_{1}= j_{1}   ,j_{2}=(j_{2}-1)\Bigg\rangle
\end{equation*}
So we can obtain all the states with $J=j_{1}+j_{2}$, $J \geq  m_{1} \geq -J $ by successively applying the ladder operator
in this manner.\\

\noindent Now we must move onto states where $J= j_{1}+j_{2}-1$. There are only two product kets from which we may construct the
coupled basis; those with $| j_{1}=j_{1}, m_{1}=j_{1}; j_{2}=j_{2}, m_{2} = j_{2}-1\rangle $and  
$| j_{1}=j_{1}, m_{1}=j_{1}-1; j_{2}=j_{2}, m_{2} = j_{2}\rangle$

\section{Appendix}
First, the  spin operators represented in the spin product basis (these are the matrices
used by EasySpin).
\begin{equation}
S(x,1) = 
\begin{bmatrix}
0                  & \frac{1}{\sqrt{2}} & 0\\
\frac{1}{\sqrt{2}} & 0                 & \frac{1}{\sqrt{2}} \\ 
0                  & \frac{1}{\sqrt{2}} & 0
\end{bmatrix}
\end{equation}
\begin{equation}
S(y,1) = 
\begin{bmatrix}
0                  & \frac{i}{\sqrt{2}} & 0\\
\frac{-i}{\sqrt{2}} & 0                 & \frac{-i}{\sqrt{2}} \\ 
0                  & \frac{i}{\sqrt{2}} & 0
\end{bmatrix}
\end{equation}
\begin{equation}
S(z,1) = 
\begin{bmatrix}
-1                  & 0 & 0\\
0 & 0               & 0    \\ 
0                   &   & 1
\end{bmatrix}
\end{equation}
Now for the product operators, $\hat{s}_{i}\otimes\hat{s}_{j}$, represented in the
spin product basis.
\begin{equation}
S_{xx} = 
\begin{bmatrix}
\frac{1}{2} & 0  & \frac{1}{2} \\ 
0           & 1 & 0\\
\frac{1}{2} & 0  & \frac{1}{2} 
\end{bmatrix}
\end{equation}

\begin{equation}
s_{xy} = 
\begin{bmatrix}
\frac{-i}{2} & 0  & \frac{i}{2} \\ 
0           & 1 & 0\\
\frac{-i}{2} & 0  & \frac{i}{2} 
\end{bmatrix}
\end{equation}

\begin{equation}
S_{xz} = 
\begin{bmatrix}
0           & 0 & 0\\
\frac{1}{2} & 0  & \frac{1}{2} \\ 
0           & 0 & 0\\
\end{bmatrix}
\end{equation}


\begin{equation}
s_{yx}
\begin{bmatrix}
\frac{i}{2} & 0  & \frac{i}{2} \\ 
0           & 1 & 0\\
\frac{-i}{2} & 0  & \frac{-i}{2} 
\end{bmatrix}
\end{equation}

\begin{equation}
s_{yy} = 
\begin{bmatrix}
0           & 0 & 0\\
\frac{1}{2} & 0  & \frac{1}{2} \\ 
0           & 0 & 0\\
\end{bmatrix}
\end{equation}
\begin{equation}
s_{yz} = 
\begin{bmatrix}
0           & 0 & 0\\
\frac{1}{2} & 0  & \frac{1}{2} \\ 
0           & 0 & 0\\


\frac{1}{2}  & 0  & \frac{-1}{2} \\ 
0            & 1  & 0\\
\frac{-1}{2} & 0  & \frac{1}{2} 
\end{bmatrix}
\end{equation}

\begin{equation}
s_{zx}
\begin{bmatrix}
\frac{i}{2} & 0  & \frac{i}{2} \\ 
0           & 1 & 0\\
\frac{-i}{2} & 0  & \frac{-i}{2} 
\end{bmatrix}
\end{equation}

\begin{equation}
s_{zy} = 
\begin{bmatrix}
0     &  \frac{-i}{\sqrt{2}} & 0 \\ 
0     & 0                    & 0 \\
0     &  \frac{-i}{\sqrt{2}} & 0 \\
\end{bmatrix}
\end{equation}
\begin{equation}
s_{zz} = 
\begin{bmatrix}
1     & 0 & 0\\
0     & 0 & 0 \\ 
0     & 0 & 1\\
\end{bmatrix}
\end{equation}



\end{document}
